c_stubs/common_tcp_karamel.h
@@ -1,0 +1,10 @@
+#ifndef COMMON_TCP_KARAMEL_H
+#define COMMON_TCP_KARAMEL_H
+
+#include <stddef.h>
+#include <stdint.h>
+
+typedef struct Common_TCP_channel_s *Common_TCP_channel;
+typedef struct Common_TCP_listener_s *Common_TCP_listener;
+
+#endif
